Add the remaining `Slice` theorems
This commit includes theorems for all of the remaining functionality for
`std::slice::Slice` that had not been previously proved. It also
contains a minor re-organization of the existing slice theorems to
better match the order in which the corresponding functions occur in the
extracted file.

Co-authored-by: Marcin Kostrzewa <marckostrzewa@gmail.com>

stdlib/lampe/Stdlib/Append.lean
@@ -2,6 +2,7 @@ import «std-1.0.0-beta.12».Extracted
 import Lampe
 
 import Stdlib.Slice
+import Stdlib.TraitMethods
 
 namespace Lampe.Stdlib.Append
 
@@ -10,32 +11,6 @@ open Lampe.Stdlib
 
 set_option Lampe.pp.Expr true
 set_option Lampe.pp.STHoare true
-
-/-- A shorthand for a call to the `std::append::Append::empty` method. -/
-@[reducible]
-def empty {p}
-    (generics : HList Kind.denote «std-1.0.0-beta.12::append::Append».«#genericKinds»)
-    (Self : Tp)
-    (associatedTypes : HList Kind.denote «std-1.0.0-beta.12::append::Append».«#associatedTypesKinds»)
-    (fnGenerics : HList Kind.denote «std-1.0.0-beta.12::append::Append».«#genericKinds»)
-  : HList (Tp.denote p)
-      («std-1.0.0-beta.12::append::Append».empty.«#inputs» generics Self associatedTypes fnGenerics)
-  → Expr (Tp.denote p)
-      («std-1.0.0-beta.12::append::Append».empty.«#output» generics Self associatedTypes fnGenerics) :=
-  «std-1.0.0-beta.12::append::Append».empty generics Self associatedTypes fnGenerics
-
-/-- A shorthand for a call to the `std::append::Append::append` method. -/
-@[reducible]
-def append {p}
-    (generics : HList Kind.denote «std-1.0.0-beta.12::append::Append».«#genericKinds»)
-    (Self : Tp)
-    (associatedTypes : HList Kind.denote «std-1.0.0-beta.12::append::Append».«#associatedTypesKinds»)
-    (fnGenerics : HList Kind.denote «std-1.0.0-beta.12::append::Append».«#genericKinds»)
-  : HList (Tp.denote p)
-      («std-1.0.0-beta.12::append::Append».append.«#inputs» generics Self associatedTypes fnGenerics)
-  → Expr (Tp.denote p)
-      («std-1.0.0-beta.12::append::Append».append.«#output» generics Self associatedTypes fnGenerics) :=
-  «std-1.0.0-beta.12::append::Append».append generics Self associatedTypes fnGenerics
 
 theorem slice_empty_spec {p T }
   : STHoare p env ⟦⟧
