stdlib/lampe/Stdlib/Slice.lean
@@ -1,5 +1,7 @@
 import «std-1.0.0-beta.12».Extracted
 import Lampe
+import Stdlib.List
+import Stdlib.TraitMethods
 
 namespace Lampe.Stdlib.Slice
 open «std-1.0.0-beta.12»
@@ -29,42 +31,59 @@ theorem append_spec {p T a b}
   · steps
     simp_all
 
-lemma for_each_inv {T Env p f fb l}
-    (Inv: List (Tp.denote p T) → SLP (State p))
-    (h_inv: ∀(lp: List (Tp.denote p T)) (e: T.denote p),
-      ((lp ++ [e]) <+: l) → STHoare p env (Inv lp) (fb h![e]) (fun _ => Inv (lp ++ [e])))
-  : STHoare p env
-    (Inv [] ⋆ [λf ↦ fb])
-    ((«std-1.0.0-beta.12::slice::for_each».call h![T, Env] h![l, f]))
-      (fun _ => Inv l ⋆ [λf ↦ fb]) := by
+theorem as_array_spec {p T N input}
+  : STHoare p env ⟦⟧
+    («std-1.0.0-beta.12::slice::as_array».call h![T, N] h![input])
+    (fun r => r.toList = input) := by
   enter_decl
-  steps []
-  loop_inv nat fun i _ _ => Inv (l.take i) ⋆ [λf ↦ fb]
-  · simp
-  · intro i ihl ihg
-    steps
-    simp_all only [BitVec.toNat_intCast, Int.reducePow, EuclideanDomain.zero_mod, Int.toNat_zero,
-      zero_le, Builtin.instCastTpU, BitVec.natCast_eq_ofNat, BitVec.ofNat_toNat, BitVec.setWidth_eq,
-      BitVec.toNat_ofNatLT, List.get_eq_getElem]
-    generalize_proofs
-    have := h_inv (l.take i) l[i] $ by
-      simp [List.take_prefix]
-    steps [STHoare.callLambda_intro (hlam := this)]
-    simp only [List.take_append_getElem]
-    sl
   steps
-  simp_all
-  sl
+  loop_inv nat fun i hlo hhi => ∃∃v, [array ↦ ⟨T.array N, v⟩] ⋆ (v.toList.take i = input.take i)
+  · sl; simp
+  · simp
+  · intro i _ _
+    steps
+    simp_all only [beq_true, decide_eq_true_eq, BitVec.toNat_intCast, Int.reducePow,
+      EuclideanDomain.zero_mod, Int.toNat_zero, zero_le, Lens.modify, Lens.get, Access.modify,
+      BitVec.toNat_ofNatLT, ↓reduceDIte, Builtin.instCastTpU, BitVec.natCast_eq_ofNat,
+      BitVec.ofNat_toNat, BitVec.setWidth_eq, List.get_eq_getElem, Option.bind_eq_bind,
+      Option.bind_some, Option.bind_fun_some, Option.get_some, List.Vector.toList_set]
+    rename_i take_of_vec_eq_input
+    rw [List.take_succ]
+    rw [List.take_set]
+    rw [take_of_vec_eq_input]
+    simp_all only [Lens.modify, Lens.get, Access.modify, BitVec.toNat_ofNatLT, ↓reduceDIte,
+      Builtin.instCastTpU, BitVec.natCast_eq_ofNat, BitVec.ofNat_toNat, BitVec.setWidth_eq,
+      List.get_eq_getElem, Option.bind_eq_bind, Option.bind_some, Option.bind_fun_some,
+      Option.isSome_some, List.length_set, List.Vector.toList_length, getElem?_pos,
+      List.getElem_set_self, Option.toList_some]
 
-lemma slice_map_inv {T U Env p f fb l}
-    (Inv: List (Tp.denote p T) → List (Tp.denote p U) → SLP (State p))
-    (h_inv: ∀(ip: List (Tp.denote p T)) (rp: List (Tp.denote p U)) (e: T.denote p),
+    have : i < input.length := by simp_all
+    have h : (List.take i input).set i input[i] = List.take i input := by
+      rw [List.set_eq_of_length_le (by simp_all)]
+    rw [h, List.take_append_getElem]
+
+  steps
+  rename_i a v _
+  subst_vars
+  have h1 : input.length = BitVec.toNat N := by aesop
+  have h2 : v.toList.length = BitVec.toNat N := by simp_all
+  conv at a =>
+    congr
+    · arg 1; rw [←h2]
+    · rw [←h1]
+
+  rw [List.take_length] at a
+  simp_all
+
+theorem map_spec {T U Env p f fb l}
+    (Inv : List (Tp.denote p T) → List (Tp.denote p U) → SLP (State p))
+    (h_inv : ∀(ip : List (Tp.denote p T)) (rp : List (Tp.denote p U)) (e : T.denote p),
       ((ip ++ [e]) <+: l) → STHoare p env (Inv ip rp) (fb h![e])
         (fun r => Inv (ip ++ [e]) (rp ++ [r])))
   : STHoare p env
     (Inv [] [] ⋆ [λf ↦ fb])
-      ((«std-1.0.0-beta.12::slice::map».call h![T, U, Env] h![l, f]))
-        (fun v => Inv l v ⋆ [λf ↦ fb]) := by
+    («std-1.0.0-beta.12::slice::map».call h![T, U, Env] h![l, f])
+    (fun v => Inv l v ⋆ [λf ↦ fb]) := by
   enter_decl
   steps
   step_as ([ret ↦ ⟨U.slice, []⟩] ⋆ [λf ↦ fb] ⋆ Inv [] [])
@@ -91,13 +110,495 @@ lemma slice_map_inv {T U Env p f fb l}
   simp_all
   sl
 
-lemma slice_pure_map {T U Env p f fb func l}
+theorem map_pure_spec {T U Env p f fb func l}
     (h_pure : ∀x, STHoare p env ⟦⟧ (fb h![x]) (fun r => r = func x))
   : STHoare p env [λf ↦ fb]
-    ((«std-1.0.0-beta.12::slice::map».call h![T, U, Env] h![l, f]))
+    («std-1.0.0-beta.12::slice::map».call h![T, U, Env] h![l, f])
     (fun v => v = l.map func) := by
-  steps [slice_map_inv (Inv := fun i o => o = i.map func)]
+  steps [map_spec (Inv := fun i o => o = i.map func)]
   · rfl
   · assumption
   · intros; steps [h_pure]; simp_all
+
+theorem mapi_spec {T U Env p f fb l}
+    (inv : List (T.denote p) → List (U.denote p) → SLP (State p))
+    (inv_sem : ∀(ip : List (T.denote p)) (op : List (U.denote p)) (e : T.denote p),
+      ((ip ++ [e]) <+: l) → STHoare p env (inv ip op) (fb h![ip.length, e])
+        (fun r => inv (ip ++ [e]) (op ++ [r])))
+  : STHoare p env
+    (inv [] [] ⋆ [λf ↦ fb])
+    («std-1.0.0-beta.12::slice::mapi».call h![T, U, Env] h![l, f])
+    (fun v => inv l v ⋆ [λf ↦ fb]) := by
+  enter_decl
+  steps
+  step_as ([ret ↦ ⟨U.slice, []⟩] ⋆ [index ↦ ⟨.u 32, 0⟩] ⋆ [λf ↦ fb] ⋆ inv [] [])
+    (fun _ => ∃∃v, [ret ↦ ⟨U.slice, v⟩] ⋆ [index ↦ ⟨.u 32, l.length⟩] ⋆ [λf ↦ fb] ⋆ inv l v)
+  · steps
+    loop_inv nat fun i _ _ =>
+      ∃∃v, [ret ↦ ⟨U.slice, v⟩] ⋆ [index ↦ ⟨.u 32, i⟩] ⋆ [λf ↦ fb] ⋆ (inv (l.take i) v)
+    · sl
+    · simp
+    · intro i hlo hhi
+      steps
+      simp_all only [BitVec.natCast_eq_ofNat, BitVec.toNat_intCast, Int.reducePow,
+        EuclideanDomain.zero_mod, Int.toNat_zero, zero_le, Builtin.instCastTpU,
+        BitVec.truncate_eq_setWidth, BitVec.setWidth_eq, BitVec.toNat_ofNatLT, List.get_eq_getElem]
+      generalize_proofs
+      rename Tp.denote p U.slice => v
+      have := inv_sem (l.take i) v l[i] (by simp [List.take_prefix])
+      have i_eq_len : (l.take i).length = i := by simp only [List.length_take, inf_eq_left]; omega
+      rw [i_eq_len] at this
+      steps [STHoare.callLambda_intro (hlam := this)]
+      · simp only [List.take_append_getElem, Lens.modify, Option.get_some]; sl
+
+      congr 1
+      simp_all only [List.take_append_getElem, List.length_take, inf_eq_left, Lens.modify,
+        Option.isSome_some, BitVec.toNat_ofNat, Nat.reducePow, BitVec.toNat_intCast, Int.reducePow,
+        Int.reduceMod, Int.toNat_one, Option.get_some]
+      rw [BitVec.ofNat_add]
+      rfl
+
+    · steps
+      · simp_all only [BitVec.natCast_eq_ofNat, BitVec.toNat_intCast, Int.reducePow,
+        EuclideanDomain.zero_mod, Int.toNat_zero, BitVec.toNat_ofNatLT, zero_le, List.take_length]
+        sl
+
+      simp_all
+
+  steps
+  simp_all only [BitVec.natCast_eq_ofNat]; sl
+
+theorem mapi_pure_spec {T U Env p f fb fEmb l}
+    (inv_pure : ∀i x, (h : i < l.length) → STHoare p env ⟦⟧ (fb h![i, x]) (fun r => r = fEmb i x))
+  : STHoare p env [λf ↦ fb]
+    («std-1.0.0-beta.12::slice::mapi».call h![T, U, Env] h![l, f])
+    (fun v => v = l.mapIdx fEmb) := by
+  steps [mapi_spec (inv := fun i o => o = i.mapIdx fEmb)]
+  · rfl
+  · assumption
+  · intros
+    rename List (T.denote p) => ip
+    rename T.denote p => e
+    steps [inv_pure ip.length e ?lt]
+    case lt =>
+      rename_i a
+      simp_all only [BitVec.natCast_eq_ofNat, List.length_cons, List.length_nil, zero_add, gt_iff_lt]
+      have h1 : (ip ++ [e]).length ≤ l.length := List.IsPrefix.length_le a
+      rw [List.length_append] at h1
+      exact h1
+
+    simp_all
+
+theorem for_each_spec {T Env p f fb l}
+    (Inv : List (Tp.denote p T) → SLP (State p))
+    (h_inv : ∀(lp: List (Tp.denote p T)) (e: T.denote p),
+      ((lp ++ [e]) <+: l) → STHoare p env (Inv lp) (fb h![e]) (fun _ => Inv (lp ++ [e])))
+  : STHoare p env
+    (Inv [] ⋆ [λf ↦ fb])
+    («std-1.0.0-beta.12::slice::for_each».call h![T, Env] h![l, f])
+    (fun _ => Inv l ⋆ [λf ↦ fb]) := by
+  enter_decl
+  steps []
+  loop_inv nat fun i _ _ => Inv (l.take i) ⋆ [λf ↦ fb]
+  · simp
+  · intro i ihl ihg
+    steps
+    simp_all only [BitVec.toNat_intCast, Int.reducePow, EuclideanDomain.zero_mod, Int.toNat_zero,
+      zero_le, Builtin.instCastTpU, BitVec.natCast_eq_ofNat, BitVec.ofNat_toNat, BitVec.setWidth_eq,
+      BitVec.toNat_ofNatLT, List.get_eq_getElem]
+    generalize_proofs
+    have := h_inv (l.take i) l[i] $ by
+      simp [List.take_prefix]
+    steps [STHoare.callLambda_intro (hlam := this)]
+    simp only [List.take_append_getElem]
+    sl
+  steps
+  simp_all
+  sl
+
+theorem for_eachi_spec {T Env p f fb l}
+    (inv : List (T.denote p) → SLP (State p))
+    (inv_spec : ∀(ip : List (T.denote p)) (e : T.denote p),
+      ((ip ++ [e]) <+: l) → STHoare p env (inv ip) (fb h![ip.length, e]) (fun _ => inv (ip ++ [e])))
+  : STHoare p env
+    (inv [] ⋆ [λf ↦ fb])
+    («std-1.0.0-beta.12::slice::for_eachi».call h![T, Env] h![l, f])
+    (fun _ => inv l ⋆ [λf ↦ fb]) := by
+  enter_decl
+  steps
+  loop_inv nat fun i _ _ => [index ↦ ⟨.u 32, i⟩] ⋆ [λf ↦ fb] ⋆ inv (l.take i)
+  · sl; simp
+  · intro i hlo hhi
+    steps
+    simp_all only [BitVec.natCast_eq_ofNat, BitVec.toNat_intCast, Int.reducePow,
+      EuclideanDomain.zero_mod, Int.toNat_zero, zero_le, Builtin.instCastTpU,
+      BitVec.truncate_eq_setWidth, BitVec.setWidth_eq, BitVec.toNat_ofNatLT, List.get_eq_getElem]
+    generalize_proofs
+    have := inv_spec (l.take i) l[i] (by simp [List.take_prefix])
+    have i_eq_len : (l.take i).length = i := by simp only [List.length_take, inf_eq_left]; omega
+    rw [i_eq_len] at this
+
+    steps [STHoare.callLambda_intro (hlam := this)]
+    · simp only [List.take_append_getElem]; sl
+
+    congr 1
+    simp_all only [List.take_append_getElem, List.length_take, inf_eq_left, Lens.modify,
+      Option.isSome_some, BitVec.toNat_ofNat, Nat.reducePow, BitVec.toNat_intCast, Int.reducePow,
+      Int.reduceMod, Int.toNat_one, Option.get_some]
+    rw [BitVec.ofNat_add]
+    rfl
+
+  steps
+  simp_all only [BitVec.natCast_eq_ofNat, BitVec.toNat_intCast, Int.reducePow,
+    EuclideanDomain.zero_mod, Int.toNat_zero, BitVec.toNat_ofNatLT, zero_le, List.take_length]
+  sl
+
+theorem fold_spec {p T U Env l a f fb}
+    (inv : List (T.denote p) → U.denote p → SLP (State p))
+    (inv_spec : ∀(ip : List (T.denote p)) (accum : U.denote p) (e : T.denote p),
+      ((ip ++ [e] <+: l) → STHoare p env (inv ip accum)
+        (fb h![accum, e])
+        (fun r => inv (ip ++ [e]) r)))
+  : STHoare p env
+    (inv [] a ⋆ [λf ↦ fb])
+    («std-1.0.0-beta.12::slice::fold».call h![T, U, Env] h![l, a, f])
+    (fun r => (inv l r) ⋆ [λf ↦ fb]) := by
+  enter_decl
+  steps
+  step_as ([accumulator ↦ ⟨U, a⟩] ⋆ [λf ↦ fb] ⋆ inv [] a)
+    (fun _ => ∃∃v, [accumulator ↦ ⟨U, v⟩] ⋆ [λf ↦ fb] ⋆ inv l v)
+  · steps
+    loop_inv nat fun i _ _ => ∃∃v, [accumulator ↦ ⟨U, v⟩] ⋆ [λf ↦ fb] ⋆ inv (l.take i) v
+    · sl
+    · simp
+    · intro i hlo hhi
+      steps
+      simp_all only [BitVec.toNat_intCast, Int.reducePow, EuclideanDomain.zero_mod, Int.toNat_zero,
+        zero_le, Builtin.instCastTpU, BitVec.truncate_eq_setWidth, BitVec.setWidth_eq,
+        BitVec.toNat_ofNatLT, List.get_eq_getElem]
+      generalize_proofs
+      rename U.denote p => v
+      have := inv_spec (l.take i) v l[i] (by simp [List.take_prefix])
+      steps [STHoare.callLambda_intro (hlam := this)]
+      simp only [List.take_append_getElem]; sl
+
+    steps
+    simp_all only [BitVec.toNat_intCast, Int.reducePow, EuclideanDomain.zero_mod, Int.toNat_zero,
+      BitVec.toNat_ofNatLT, zero_le, List.take_length]
+    sl
+
+  steps
+  subst_vars
+  sl
+
+theorem fold_pure_spec {p T U Env l a f fb fEmb}
+    (inv_pure : ∀a x, STHoare p env ⟦⟧ (fb h![a, x]) (fun r => r = fEmb a x))
+  : STHoare p env [λf ↦ fb]
+    («std-1.0.0-beta.12::slice::fold».call h![T, U, Env] h![l, a, f])
+    (fun r => r = l.foldl fEmb a ⋆ [λf ↦ fb]) := by
+  steps [fold_spec (inv := fun xs v => v = xs.foldl fEmb a)]
+  · rfl
+  · assumption
+  · intros; steps [inv_pure]; simp_all
+
+theorem reduce_spec {p T Env l f fb}
+    (l_len_gt : l.length > 0)
+    (inv : List (T.denote p) → T.denote p → SLP (State p))
+    (inv_spec : ∀(ip : List (T.denote p)) (acc : T.denote p) (e : T.denote p),
+      ((ip ++ [e] <+: l.tail) → STHoare p env (inv ip acc) (fb h![acc, e]) (fun r => inv (ip ++ [e]) r)))
+  : STHoare p env
+    ((inv [] l[0]) ⋆ [λf ↦ fb])
+    («std-1.0.0-beta.12::slice::reduce».call h![T, Env] h![l, f])
+    (fun r => (inv l.tail r) ⋆ [λf ↦ fb]) := by
+  enter_decl
+  steps
+  cases l with
+  | nil => contradiction
+  | cons init l =>
+    simp at *
+    loop_inv nat fun i _ _ => ∃∃v, [accumulator ↦ ⟨T, v⟩] ⋆ [λf ↦ fb] ⋆ inv (l.take (i-1)) v
+    · sl
+    · simp only [BitVec.toNat_intCast, BitVec.toNat_ofNatLT]; omega
+    · intro i hlo hhi
+      cases i with
+      | zero => contradiction
+      | succ i =>
+        steps
+        simp_all only [gt_iff_lt, BitVec.toNat_intCast, Int.reducePow, EuclideanDomain.zero_mod,
+          Int.toNat_zero, Int.reduceMod, Int.toNat_one, Builtin.instCastTpU,
+          BitVec.truncate_eq_setWidth, BitVec.setWidth_eq, BitVec.toNat_ofNatLT, List.get_eq_getElem]
+        generalize_proofs
+        rename T.denote p => v
+        have := inv_spec (l.take i) v (l[i]'(by simp_all)) (by simp [List.take_prefix])
+        simp only [List.take_append_getElem] at this
+
+        steps [STHoare.callLambda_intro (hlam := this)]
+
+    steps
+    simp_all only [List.length_cons, gt_iff_lt, lt_add_iff_pos_left, add_pos_iff, zero_lt_one,
+      or_true, BitVec.toNat_intCast, Int.reducePow, EuclideanDomain.zero_mod, Int.toNat_zero,
+      Int.reduceMod, Int.toNat_one, BitVec.toNat_ofNatLT, le_add_iff_nonneg_left, zero_le,
+      add_tsub_cancel_right, List.take_length]
+    sl
+
+theorem reduce_pure_spec {p T Env l f fb fEmb}
+    (l_len_gt : l.length > 0)
+    (inv_pure : ∀a x, STHoare p env ⟦⟧ (fb h![a, x]) (fun r => r = fEmb a x))
+  : STHoare p env [λf ↦ fb]
+    («std-1.0.0-beta.12::slice::reduce».call h![T, Env] h![l, f])
+    (fun r => r = l.tail.foldl fEmb l[0] ⋆ [λf ↦ fb]) := by
+  steps [reduce_spec (inv := fun xs v => v = xs.foldl fEmb l[0])]
+  · rfl
+  · assumption
+  · intros
+    steps [inv_pure]
+    simp_all
+
+theorem filter_spec {p T Env l f fb}
+    (inv : List (T.denote p) → List (T.denote p) → SLP (State p))
+    (inv_spec : ∀(ip : List (T.denote p)) (op : List (T.denote p)) (e : T.denote p),
+      ((ip ++ [e] <+: l) → STHoare p env (inv ip op) (fb h![e])
+        (fun r => inv (ip ++ [e]) (if r then (op ++ [e]) else op))))
+  : STHoare p env
+    (inv [] [] ⋆ [λf ↦ fb])
+    («std-1.0.0-beta.12::slice::filter».call h![T, Env] h![l, f])
+    (fun r => (inv l r) ⋆ [λf ↦ fb]) := by
+  enter_decl
+  steps
+  step_as ([ret ↦ ⟨T.slice, []⟩] ⋆ [λf ↦ fb] ⋆ (inv [] []))
+    (fun _ => ∃∃v, [ret ↦ ⟨T.slice, v⟩] ⋆ [λf ↦ fb] ⋆ (inv l v))
+  · steps
+    loop_inv nat fun i _ _ => ∃∃v, [ret ↦ ⟨T.slice, v⟩] ⋆ [λf ↦ fb] ⋆ (inv (l.take i) v)
+    · sl
+    · simp
+    · intro i hlo hhi
+      steps
+      simp_all only [BitVec.toNat_intCast, Int.reducePow, EuclideanDomain.zero_mod, Int.toNat_zero,
+        zero_le, Builtin.instCastTpU, BitVec.truncate_eq_setWidth, BitVec.setWidth_eq,
+        BitVec.toNat_ofNatLT, List.get_eq_getElem]
+      generalize_proofs
+      rename Tp.denote p (T.slice) => v
+
+      have := inv_spec (l.take i) v l[i] (by simp [List.take_prefix])
+      steps [STHoare.callLambda_intro (hlam := this)]
+
+      apply STHoare.ite_intro
+      · intros
+        steps
+        simp_all
+        sl
+      · intros
+        steps
+        simp_all
+        sl
+
+    steps
+    simp_all
+    sl
+
+  steps
+  simp_all
+  sl
+
+theorem filter_pure_spec {p T Env l f fb fEmb}
+    (inv_pure : ∀x, STHoare p env ⟦⟧ (fb h![x]) (fun r => r = fEmb x))
+  : STHoare p env [λf ↦ fb]
+    («std-1.0.0-beta.12::slice::filter».call h![T, Env] h![l, f])
+    (fun r => (r = l.filter fEmb)) := by
+  steps [filter_spec (inv := fun xs v => v = xs.filter fEmb)]
+  · rfl
+  · assumption
+  · intros
+    steps [inv_pure]
+    subst_vars
+    split
+    all_goals simp_all
+
+theorem join_spec {p T a s}
+    {t_append : Append.hasImpl env T}
+    {t_empty_emb : T.denote p}
+    {t_app_emb : T.denote p → T.denote p → T.denote p}
+    (t_empty_sem : STHoare p env ⟦⟧ (Append.empty h![] T h![] h![] h![]) (fun r => r = t_empty_emb))
+    (t_app_sem : ∀a b, STHoare p env ⟦⟧ (Append.append h![] T h![] h![] h![a, b])
+      (fun r => r = t_app_emb a b))
+  : STHoare p env ⟦⟧
+    («std-1.0.0-beta.12::slice::join».call h![T] h![a, s])
+    (fun r => r = if h : a.length > 0 then
+      a.tail.foldl (fun l r => t_app_emb (t_app_emb l s) r) a[0]
+    else t_empty_emb) := by
+  enter_decl
+  steps [t_empty_sem]
+
+  let foldFnEmb := fun l r => t_app_emb (t_app_emb l s) r
+
+  step_as ([ret ↦ ⟨T, t_empty_emb⟩])
+    (fun _ => [ret ↦ ⟨T, if h : a.length > 0 then a.tail.foldl foldFnEmb a[0] else t_empty_emb⟩])
+
+  apply STHoare.ite_intro
+  · intro cond
+    steps
+    simp_all only [ne_eq, decide_not, Bool.not_eq_eq_eq_not, Bool.not_true, decide_eq_false_iff_not,
+      Lens.modify, BitVec.toNat_intCast, Int.reducePow, EuclideanDomain.zero_mod, Int.toNat_zero,
+      List.get_eq_getElem, Option.get_some, gt_iff_lt]
+
+    loop_inv nat fun i _ _ => [ret ↦ ⟨T, (a.tail.take (i - 1)).foldl foldFnEmb a[0]⟩]
+    · simp_all only [Lens.modify, BitVec.toNat_intCast, Int.reducePow, EuclideanDomain.zero_mod,
+      Int.toNat_zero, List.get_eq_getElem, Option.isSome_some, Int.reduceMod, Int.toNat_one,
+      BitVec.toNat_ofNatLT]
+      omega
+    · intro i hlo hhi
+      steps [t_app_sem]
+      congr
+      simp_all only [Lens.modify, BitVec.toNat_intCast, Int.reducePow, EuclideanDomain.zero_mod,
+        Int.toNat_zero, List.get_eq_getElem, Option.isSome_some, Int.reduceMod, Int.toNat_one,
+        Builtin.instCastTpU, BitVec.truncate_eq_setWidth, BitVec.setWidth_eq, BitVec.toNat_ofNatLT,
+        Option.get_some]
+
+      have : i + 1 - 1 = i - 1 + 1 := by omega
+      rw [this, List.take_succ_eq_append_getElem ?i_lt]
+
+      case i_lt =>
+        rw [List.length_tail]
+        have : i < a.length := by simp [BitVec.toNat_ofNatLT (by omega)] at hhi; assumption
+        omega
+
+      simp [List.getElem_tail, Nat.sub_add_cancel hlo, foldFnEmb]
+
+    steps
+    congr
+    have : 0 < a.length := by omega
+    simp_all only [Lens.modify, BitVec.toNat_intCast, Int.reducePow, EuclideanDomain.zero_mod,
+      Int.toNat_zero, List.get_eq_getElem, Option.isSome_some, Int.reduceMod, Int.toNat_one,
+      BitVec.toNat_ofNatLT, ↓reduceDIte]
+
+    congr
+    rw [←List.length_tail, List.take_length]
+
+  · intro cond
+    simp_all only [ne_eq, decide_not, Bool.not_eq_eq_eq_not, Bool.not_false, decide_eq_true_eq,
+      gt_iff_lt]
+    steps
+    congr
+    have : a.length = 0 := by
+      apply_fun BitVec.toNat at cond
+      rw [BitVec.toNat_ofNatLT (a.length) (by omega)] at cond
+      norm_cast
+    rw [List.length_eq_zero_iff.mp this]
+    simp
+
+  steps
+  simp_all [foldFnEmb]
+
+theorem all_spec {p T Env l f fb}
+    (inv : List (T.denote p) → Bool → SLP (State p))
+    (inv_spec : ∀(ip : List (T.denote p)) (op : Bool) (e : T.denote p),
+      (ip ++ [e] <+: l) → STHoare p env (inv ip op) (fb h![e]) (fun r => inv (ip ++ [e]) (op ∧ r)))
+  : STHoare p env
+    ((inv [] true) ⋆ [λf ↦ fb])
+    («std-1.0.0-beta.12::slice::all».call h![T, Env] h![l, f])
+    (fun r => (inv l r) ⋆ [λf ↦ fb]) := by
+  enter_decl
+  steps
+
+  step_as ([ret ↦ ⟨.bool, true⟩] ⋆ (inv [] true) ⋆ [λf ↦ fb])
+    (fun r => ∃∃b, [ret ↦ ⟨.bool, b⟩] ⋆ (inv l b) ⋆ [λf ↦ fb])
+
+  steps
+  loop_inv nat fun i _ _ => ∃∃b, [ret ↦ ⟨.bool, b⟩] ⋆ (inv (l.take i) b) ⋆ [λf ↦ fb]
+  · sl
+  · simp
+  · intro i hlo hhi
+    steps
+    simp_all only [BitVec.toNat_intCast, Int.reducePow, EuclideanDomain.zero_mod, Int.toNat_zero,
+      zero_le, Builtin.instCastTpU, BitVec.truncate_eq_setWidth, BitVec.setWidth_eq,
+      BitVec.toNat_ofNatLT, List.get_eq_getElem]
+
+    generalize_proofs
+    rename Tp.denote p .bool => b
+    have := inv_spec (l.take i) b l[i] (by simp [List.take_prefix])
+
+    steps [STHoare.callLambda_intro (hlam := this)]
+    · exact ()
+
+    simp_all only [Bool.decide_and, Bool.decide_eq_true, Bool.forall_bool, Bool.false_and,
+      Bool.true_and, List.take_append_getElem, Lens.modify, Option.get_some]
+    steps
+  · simp_all only [Bool.decide_and, Bool.decide_eq_true, Bool.forall_bool, Bool.false_and,
+    Bool.true_and, BitVec.toNat_ofNatLT, List.take_length, SLP.star_true]
+    steps
+
+  steps
+  subst_vars
+  sl
+
+theorem all_pure_spec {p T Env l f fb fEmb}
+    (inv_pure : ∀a, STHoare p env ⟦⟧ (fb h![a]) (fun r => r = fEmb a))
+  : STHoare p env [λf ↦ fb]
+    («std-1.0.0-beta.12::slice::all».call h![T, Env] h![l, f])
+    (fun r => r = l.all fEmb) := by
+  steps [all_spec (inv := fun x r => r = x.all fEmb)]
+  · simp
+  · assumption
+  · intro ip op e pfx
+    steps [inv_pure]
+    simp_all only [List.all_eq_true, Bool.decide_and, Bool.decide_eq_true, List.all_append,
+      List.all_cons, List.all_nil, Bool.and_true]
+    rw [←List.all_eq]
+
+theorem any_spec {p T Env l f fb}
+    (inv : List (T.denote p) → Bool → SLP (State p))
+    (inv_spec : ∀(ip : List (T.denote p)) (op : Bool) (e : T.denote p),
+      (ip ++ [e] <+: l) → STHoare p env (inv ip op) (fb h![e]) (fun r => inv (ip ++ [e]) (op ∨ r)))
+  : STHoare p env
+    ((inv [] false) ⋆ [λf ↦ fb])
+    («std-1.0.0-beta.12::slice::any».call h![T, Env] h![l, f])
+    (fun r => (inv l r) ⋆ [λf ↦ fb]) := by
+  enter_decl
+  steps
+
+  step_as ([ret ↦ ⟨.bool, false⟩] ⋆ (inv [] false) ⋆ [λf ↦ fb])
+    (fun r => ∃∃b, [ret ↦ ⟨.bool, b⟩] ⋆ (inv l b) ⋆ [λf ↦ fb])
+
+  steps
+  loop_inv nat fun i _ _ => ∃∃b, [ret ↦ ⟨.bool, b⟩] ⋆ (inv (l.take i) b) ⋆ [λf ↦ fb]
+  · sl
+  · simp
+  · intro i hlo hhi
+    steps
+    simp_all only [BitVec.toNat_intCast, Int.reducePow, EuclideanDomain.zero_mod, Int.toNat_zero,
+      zero_le, Builtin.instCastTpU, BitVec.truncate_eq_setWidth, BitVec.setWidth_eq,
+      BitVec.toNat_ofNatLT, List.get_eq_getElem]
+
+    generalize_proofs
+    rename Tp.denote p .bool => b
+    have := inv_spec (l.take i) b l[i] (by simp [List.take_prefix])
+
+    steps [STHoare.callLambda_intro (hlam := this)]
+    · exact ()
+
+    simp_all only [Bool.decide_or, Bool.decide_eq_true, Bool.forall_bool, Bool.false_or,
+      Bool.true_or, List.take_append_getElem, Lens.modify, Option.get_some]
+    steps
+
+  · simp_all only [Bool.decide_or, Bool.decide_eq_true, Bool.forall_bool, Bool.false_or, Bool.true_or,
+    BitVec.toNat_ofNatLT, List.take_length, SLP.star_true]
+    steps
+
+  steps
+  subst_vars
+  sl
+
+theorem any_pure_spec {p T Env l f fb fEmb}
+    (inv_pure : ∀a, STHoare p env ⟦⟧ (fb h![a]) (fun r => r = fEmb a))
+  : STHoare p env [λf ↦ fb]
+    («std-1.0.0-beta.12::slice::any».call h![T, Env] h![l, f])
+    (fun r => r = l.any fEmb) := by
+  steps [any_spec (inv := fun x r => r = x.any fEmb)]
+  · simp
+  · assumption
+  · intro ip op e pfx
+    steps [inv_pure]
+    simp_all only [List.any_eq_true, Bool.decide_or, Bool.decide_eq_true, List.any_append,
+      List.any_cons, List.any_nil, Bool.or_false]
+    rw [←List.any_eq]
 
