stdlib/lampe/Stdlib/Stdlib.lean
@@ -27,6 +27,7 @@ import Stdlib.Panic
 import Stdlib.Slice
 import Stdlib.String
 import Stdlib.Tp
+import Stdlib.TraitMethods
 import Stdlib.Tuple
 
 import «std-1.0.0-beta.12».Extracted
