stdlib/lampe/Stdlib/TraitMethods.lean
@@ -1,0 +1,52 @@
+import «std-1.0.0-beta.12».Extracted
+import Lampe
+
+/-!
+This file contains (namespaced) definitions of shorthand for calling various trait methods, as well
+as asserting the existence of certain trait implementations on types.
+
+Where possible, these shorthands should live in the corresponding files (e.g. `Eq::eq`'s shorthand
+is in `Cmp.lean`), but in some cases the potential for import cycles can require that they are
+pulled out into a separate file. This is that file.
+-/
+
+namespace Lampe.Stdlib
+
+open «std-1.0.0-beta.12»
+open Lampe.Stdlib
+
+namespace Append
+
+/-- A shorthand for a call to the `std::append::Append::empty` method. -/
+@[reducible]
+def empty {p}
+    (generics : HList Kind.denote «std-1.0.0-beta.12::append::Append».«#genericKinds»)
+    (Self : Tp)
+    (associatedTypes : HList Kind.denote «std-1.0.0-beta.12::append::Append».«#associatedTypesKinds»)
+    (fnGenerics : HList Kind.denote «std-1.0.0-beta.12::append::Append».«#genericKinds»)
+  : HList (Tp.denote p)
+      («std-1.0.0-beta.12::append::Append».empty.«#inputs» generics Self associatedTypes fnGenerics)
+  → Expr (Tp.denote p)
+      («std-1.0.0-beta.12::append::Append».empty.«#output» generics Self associatedTypes fnGenerics) :=
+  «std-1.0.0-beta.12::append::Append».empty generics Self associatedTypes fnGenerics
+
+/-- A shorthand for a call to the `std::append::Append::append` method. -/
+@[reducible]
+def append {p}
+    (generics : HList Kind.denote «std-1.0.0-beta.12::append::Append».«#genericKinds»)
+    (Self : Tp)
+    (associatedTypes : HList Kind.denote «std-1.0.0-beta.12::append::Append».«#associatedTypesKinds»)
+    (fnGenerics : HList Kind.denote «std-1.0.0-beta.12::append::Append».«#genericKinds»)
+  : HList (Tp.denote p)
+      («std-1.0.0-beta.12::append::Append».append.«#inputs» generics Self associatedTypes fnGenerics)
+  → Expr (Tp.denote p)
+      («std-1.0.0-beta.12::append::Append».append.«#output» generics Self associatedTypes fnGenerics) :=
+  «std-1.0.0-beta.12::append::Append».append generics Self associatedTypes fnGenerics
+
+/--
+Asserts that the provided `tp` has an implementation of `std::append::Append` in the environment.
+-/
+@[reducible]
+def hasImpl (env : Env) (tp : Tp) := «std-1.0.0-beta.12::append::Append».hasImpl env h![] tp
+
+end Append
